Complete stabilizing functions

theories/Tools.v
@@ -1,25 +1,36 @@
 From Ltac2 Require Export Ltac2.
 From Stdlib Require Export Unicode.Utf8.
+From Stdlib Require Export Logic.Classical.
 From Stdlib Require Export Logic.FunctionalExtensionality.
 From Stdlib Require Export Logic.PropExtensionality.
+From Stdlib Require Export Logic.IndefiniteDescription.
 From Stdlib Require Arith.Arith.
 From Stdlib Require Export ZArith.ZArith.
 From Stdlib Require Export micromega.Lia.
 From Stdlib Require Lists.List.
 Export Stdlib.Lists.List.ListNotations.
 From Corelib Require Export Program.Basics.
+(* From Corelib Require Export Program.Utils. *)
 From Stdlib Require Export Classes.EquivDec.
+From Stdlib Require Export Sorting.Sorted.
 
 #[global] Obligation Tactic := ().
 Unset Program Cases.
+Unset Program Generalized Coercion.
+Unset Implicit Arguments.
 
+Ltac2 Notation "lia" := ltac1:(lia).
+
+Open Scope program_scope.
 Open Scope equiv_scope.
+Open Scope bool_scope.
 Open Scope list_scope.
 Open Scope Z_scope.
 Open Scope nat_scope.
 
 Disable Notation "_ ≤ _".
 Disable Notation "_ ≥ _".
+(* Disable Notation "{ ( _ , _ ) : _ | _ }". *)
 
 Notation "x ≤ y" := (le x y) : nat_scope.
 Notation "x ≥ y" := (ge x y) : nat_scope.
@@ -33,7 +44,418 @@ Notation "x ≤ y ≤ z" := (x ≤ y /\ y ≤ z)%Z : Z_scope.
 Notation "x ≤ y < z" := (x ≤ y /\ y < z)%Z : Z_scope.
 Notation "x < y ≤ z" := (x < y /\ y ≤ z)%Z : Z_scope.
 
+Notation " ! " := (False_rect _ _) : program_scope. (* copied from Corelib.Program.Utils *)
+
+Notation " ` t " := (proj1_sig t) (at level 10, t at next level) : program_scope. (* copied from Corelib.Program.Utils *)
+
 Instance dec_eq_Z : EqDec Z eq := Z.eq_dec.
+
+Class Total {A} (R : A → A → Prop) :=
+  | totality : ∀ x y, R x y ∨ R y x.
+
+Instance total_nat_le : Total Nat.le := Nat.le_ge_cases.
+
+Instance total_Z_le : Total Z.le := Z.le_ge_cases.
+
+Definition le {A} {R : A → A → Prop} {pre_order_R : PreOrder R} := R.
+
+Declare Scope le_scope.
+Delimit Scope le_scope with le.
+
+Notation "x <= y" := (le x y) (at level 70, no associativity) : le_scope.
+Notation "x ≤ y" := (le x y) (at level 70, no associativity) : le_scope.
+
+Class DecLe {A} (R : A → A → Prop) {pre_order_R : PreOrder R} :=
+  | dec_le : ∀ x y : A, { (x ≤ y)%le } + { ¬ (x ≤ y)%le }.
+
+Notation "x <=? y" := (dec_le x y) (at level 70, no associativity) : le_scope.
+Notation "x ≤? y" := (dec_le x y) (at level 70, no associativity) : le_scope.
+
+Instance dec_le_nat : DecLe Nat.le := le_dec.
+
+Instance dec_le_Z : DecLe Z.le := Z_le_dec.
+
+#[program]
+Instance dec_le_impl_dec_eq {A} (R : A → A → Prop) {pre_order_R : PreOrder R} {partial_order_R : PartialOrder eq R} {total_R : Total R} {dec_le_R : DecLe R} : EqDec A eq :=
+  λ x y,
+    match (x ≤? y)%le, (y ≤? x)%le with
+    | left _, left _ => left _
+    | left _, right _ => right _
+    | right _, left _ => right _
+    | right _, right _ => right _
+    end.
+Next Obligation.
+  intros A R pre_order_R partial_order_R total_R dec_le_R x y H_x_y H_y_x. apply partial_order_equivalence. split; auto.
+Qed.
+Next Obligation.
+  intros A R pre_order_R partial_order_R total_R dec_le_R x y H_x_y H_y_x. unfold equiv. intros <-. auto.
+Qed.
+Next Obligation.
+  intros A R pre_order_R partial_order_R total_R dec_le_R x y H_x_y H_y_x. unfold equiv. intros <-. auto.
+Qed.
+Next Obligation.
+  intros A R pre_order_R partial_order_R total_R dec_le_R x y H_x_y H_y_x. exfalso. destruct (totality x y); auto.
+Qed.
+
+Definition max {A} {R : A → A → Prop} {pre_order_R : PreOrder R} {dec_le_R : DecLe R} (x y : A) :=
+  if (x ≤? y)%le then y else x.
+
+Lemma commutative_max {A} (R : A → A → Prop) {pre_order_R : PreOrder R} {partial_order_R : PartialOrder eq R} {total_R : Total R} {dec_le_R : DecLe R} :
+  ∀ x y : A, max x y = max y x.
+Proof.
+  intros x y. unfold max. destruct (x ≤? y)%le as [H_x_y | H_x_y], (y ≤? x)%le as [H_y_x | H_y_x].
+  - apply partial_order_equivalence. split; auto.
+  - auto.
+  - auto.
+  - exfalso. destruct (totality x y); auto.
+Qed.
+
+Lemma le_max {A} {R : A → A → Prop} {pre_order_R : PreOrder R} {total_R : Total R} {dec_le_R : DecLe R} :
+  ∀ x y z : A, (max x y ≤ z)%le ↔ ((x ≤ z)%le ∧ (y ≤ z)%le).
+Proof.
+  intros x y z. unfold max. split.
+  - intros H. destruct (x ≤? y)%le as [H_x_y | H_x_y].
+    + split.
+      * apply transitivity with y; auto.
+      * auto.
+    + split.
+      * auto.
+      * destruct (totality y z) as [H_y_z | H_y_z].
+        -- auto.
+        -- exfalso. apply H_x_y. apply transitivity with z; auto.
+  - intros (H_x_z & H_y_z). destruct (x ≤? y)%le as [H_x_y | H_x_y]; auto.
+Qed.
+
+Fixpoint list_max_opt {A} {R : A → A → Prop} {pre_order_R : PreOrder R} {dec_le_R : DecLe R} (l : list A) :=
+  match l with
+  | [] => None
+  | [x] => Some x
+  | x :: l =>
+    match list_max_opt l with
+    | Some y => Some (max x y)
+    | None => Some x
+    end
+  end.
+
+Lemma list_max_opt_none {A} {R : A → A → Prop} {pre_order_R : PreOrder R} {dec_le_R : DecLe R} :
+  ∀ l : list A,
+  list_max_opt l = None →
+  l = [].
+Proof.
+  intros l H_l. destruct l as [| x l'].
+  - auto.
+  - simpl in H_l. destruct l' as [| y l''].
+    + simpl in H_l. congruence.
+    + destruct (list_max_opt (y :: l'')); congruence.
+Qed.
+
+Lemma le_list_max_opt {A} {R : A → A → Prop} {pre_order_R : PreOrder R} {total_R : Total R} {dec_le_R : DecLe R} :
+  ∀ (l : list A) x,
+  list_max_opt l = Some x →
+  ∀ y, (x ≤ y)%le ↔ (∀ z, List.In z l → (z ≤ y)%le).
+Proof.
+  intros l x H_x y. revert x H_x. induction l as [| z l' IH]; intros x H_x.
+  - simpl in H_x. congruence.
+  - simpl in H_x. simpl. destruct l' as [| z' l''].
+    + injection H_x as ->. simpl. split.
+      * intros H. intros _ [<- | []]. auto.
+      * intros H. apply H. left. auto.
+    + remember (list_max_opt (z' :: l'')) as x_opt eqn:H_x_opt. destruct x_opt as [x' |].
+      * injection H_x as <-. rewrite le_max. specialize (IH x' eq_refl). rewrite IH. split.
+        -- intros (H_1 & H_2). intros z'' [<- |]; auto.
+        -- intros H. split.
+           ++ apply H. left. auto.
+           ++ intros z'' H_z''. apply H. right. auto.
+      * symmetry in H_x_opt. apply list_max_opt_none in H_x_opt. congruence.
+Qed.
+
+Definition finite A := { l | ∀ a : A, List.In a l }.
+
+Definition infinite A := ∀ l, { a : A | ¬ List.In a l }.
+
+Lemma inhabited_finite_or_inhabited_infinite :
+  ∀ A, inhabited (finite A) ∨ inhabited (infinite A).
+Proof.
+  intros A. unfold finite, infinite. destruct (classic (∃ l, ∀ a : A, List.In a l)) as [(l & H) | H].
+  - left. exists. exists l. auto.
+  - right. exists. intros l. specialize (not_ex_all_not _ _ H l) as H'. apply not_all_ex_not in H'.
+    apply constructive_indefinite_description. auto.
+Qed.
+
+Lemma not_finite_and_infinite :
+  ∀ A, finite A → infinite A → False.
+Proof.
+  intros A (l & H_1) H_2. specialize (H_2 l) as (a & H_2). specialize (H_1 a). auto.
+Qed.
+
+Lemma not_inhabited_finite_and_inhabited_infinite :
+  ∀ A, inhabited (finite A) → inhabited (infinite A) → False.
+Proof.
+  intros A [H_1] [H_2]. apply (not_finite_and_infinite A); auto.
+Qed.
+
+Lemma not_inhabited_finite_equiv_not_inhabited_infinite :
+  ∀ A, ¬ inhabited (finite A) ↔ inhabited (infinite A).
+Proof.
+  intros A. specialize (inhabited_finite_or_inhabited_infinite A). specialize (not_inhabited_finite_and_inhabited_infinite A).
+  ltac1:(intuition auto).
+Qed.
+
+Class DecFinite A :=
+  | dec_finite : finite A + infinite A.
+
+#[program]
+Definition infinite_nat : infinite nat :=
+  λ l, exist _ (
+    match @list_max_opt _ Nat.le _ _ l with
+    | Some n => S n
+    | None => 0
+    end
+  ) _.
+Next Obligation.
+  intros l. remember (@list_max_opt _ Nat.le _ _ l) as n eqn:H_n; symmetry in H_n. destruct n as [n |].
+  - intros H. specialize (le_list_max_opt _ _ H_n) as H'_n. clear H_n. specialize (H'_n n) as (H'_n & _).
+    specialize (H'_n (reflexivity _)). specialize (H'_n _ H). unfold le in H'_n. lia.
+  - apply list_max_opt_none in H_n. subst l. auto.
+Qed.
+
+Instance dec_finite_nat : DecFinite nat := inr infinite_nat.
+
+#[program]
+Definition infinite_Z : infinite Z :=
+  λ l, exist _ (
+    match @list_max_opt _ Z.le _ _ l with
+    | Some n => (n + 1)%Z
+    | None => 0%Z
+    end
+  ) _.
+Next Obligation.
+  intros l. remember (@list_max_opt _ Z.le _ _ l) as n eqn:H_n; symmetry in H_n. destruct n as [n |].
+  - intros H. specialize (le_list_max_opt _ _ H_n) as H'_n. clear H_n. specialize (H'_n n) as (H'_n & _).
+    specialize (H'_n (reflexivity _)). specialize (H'_n _ H). unfold le in H'_n. lia.
+  - apply list_max_opt_none in H_n. subst l. auto.
+Qed.
+
+Instance dec_finite_Z : DecFinite Z := inr infinite_Z.
+
+Fixpoint list_sorted_nodup {A} {R : A → A → Prop} {pre_order_R : PreOrder R} (l : list A) :=
+  match l with
+  | [] => True
+  | [_] => True
+  | x :: ((y :: _) as l') => (x ≤ y)%le ∧ ¬ (y ≤ x)%le ∧ list_sorted_nodup l'
+  end.
+
+Fixpoint list_insert_nodup {A} {R : A → A → Prop} {pre_order_R : PreOrder R} {dec_le_R : DecLe R} (x : A) l :=
+  match l with
+  | [] => [x]
+  | y :: l' =>
+    if (x ≤? y)%le then
+      if (y ≤? x)%le then
+        y :: l'
+      else
+        x :: y :: l'
+    else
+      y :: (list_insert_nodup x l')
+  end.
+
+Definition list_sort_nodup {A} {R : A → A → Prop} {pre_order_R : PreOrder R} {dec_le_R : DecLe R} (l : list A) :=
+  List.fold_right list_insert_nodup [] l.
+
+Lemma list_In_list_insert_nodup {A} {R : A → A → Prop} {pre_order_R : PreOrder R} {partial_order_R : PartialOrder eq R} {total_R : Total R} {dec_le_R : DecLe R} :
+  ∀ (x : A) l y,
+  List.In y (list_insert_nodup x l) ↔ List.In y l ∨ x = y.
+Proof.
+  intros x l y. induction l as [| z l' IH].
+  - simpl. ltac1:(intuition auto).
+  - simpl. destruct (x ≤? z)%le as [H_x_z | H_x_z].
+    + destruct (z ≤? x)%le as [H_z_x | H_z_x].
+      * assert (H : x = z). {
+          apply partial_order_equivalence. split; auto.
+        }
+        subst z. simpl. ltac1:(intuition auto).
+      * simpl. ltac1:(intuition auto).
+    + simpl. rewrite IH. ltac1:(intuition auto).
+Qed.
+
+Lemma list_In_list_sort_nodup {A} {R : A → A → Prop} {pre_order_R : PreOrder R} {partial_order_R : PartialOrder eq R} {total_R : Total R} {dec_le_R : DecLe R} :
+  ∀ (l : list A) x,
+  List.In x (list_sort_nodup l) ↔ List.In x l.
+Proof.
+  intros l x. induction l as [| y l' IH].
+  - simpl. reflexivity.
+  - simpl. rewrite list_In_list_insert_nodup, IH. ltac1:(intuition auto).
+Qed.
+
+Lemma list_sorted_nodup_list_insert_nodup {A} {R : A → A → Prop} {pre_order_R : PreOrder R} {partial_order_R : PartialOrder eq R} {total_R : Total R} {dec_le_R : DecLe R} :
+  ∀ (x : A) l,
+  list_sorted_nodup l →
+  list_sorted_nodup (list_insert_nodup x l).
+Proof.
+  intros x l H_l. induction l as [| y l' IH].
+  - auto.
+  - simpl in H_l |- *. destruct (x ≤? y)%le as [H_x_y | H_x_y].
+    + destruct (y ≤? x)%le as [H_y_x | H_y_x].
+      * simpl. auto.
+      * simpl. repeat split; auto.
+    + assert (H_y_x : (y ≤ x)%le). {
+        destruct (totality y x) as [H | H].
+        - auto.
+        - exfalso. apply H_x_y. auto.
+      }
+      destruct l' as [| z l''].
+      * simpl. repeat split; auto.
+      * destruct H_l as (H_y_z & H_z_y & H_l'). specialize (IH H_l'). simpl in IH |- *. destruct (x ≤? z)%le as [H_x_z | H_x_z].
+        -- destruct (z ≤? x)%le as [H_z_x | H_z_x].
+           ++ split; auto.
+           ++ remember (z :: l'') as l'; simpl; subst l'. repeat split; auto.
+        -- repeat split; auto.
+Qed.
+
+Lemma list_sorted_nodup_list_sort_nodup {A} {R : A → A → Prop} {pre_order_R : PreOrder R} {partial_order_R : PartialOrder eq R} {total_R : Total R} {dec_le_R : DecLe R} :
+  ∀ l : list A,
+  list_sorted_nodup (list_sort_nodup l).
+Proof.
+  intros l. induction l as [| x l' IH].
+  - simpl. auto.
+  - simpl. apply list_sorted_nodup_list_insert_nodup. auto.
+Qed.
+
+Lemma list_sorted_nodup_impl_not_list_in {A} {R : A → A → Prop} {pre_order_R : PreOrder R} {partial_order_R : PartialOrder eq R} {total_R : Total R} :
+  ∀ (x : A) l,
+  list_sorted_nodup (x :: l) →
+  ∀ y,
+  (y ≤ x)%le →
+  ¬ (x ≤ y)%le →
+  ¬ List.In y (x :: l).
+Proof.
+  intros x l. simpl. revert x. induction l as [| z l' IH]; intros x H_x_l y H_y_x H_x_y.
+  - simpl. intros [<- | H_y]; auto.
+  - destruct (H_x_l) as (H_x_z & H_z_x & H_z_l'). simpl in H_z_l' |- *. destruct l' as [| w l''].
+    + intros [<- | [<- | H_y]]; auto.
+    + destruct H_z_l' as (H_z_w & H_w_z & h_w_l''). intros [<- | [<- | H_y]].
+      * auto.
+      * auto.
+      * assert (H_y_z : (y ≤ z)%le). {
+          apply transitivity with x; auto.
+        }
+        assert (H_z_y : ¬ (z ≤ y)%le). {
+          intros H_z_y.
+          assert (H : z = y). {
+            apply partial_order_equivalence. split; auto.
+          }
+          subst z. auto.
+        }
+        specialize (IH z ltac:(auto) y H_y_z H_z_y). apply IH. right. auto.
+Qed.
+
+Lemma list_sorted_nodup_impl_canonical {A} {R : A → A → Prop} {pre_order_R : PreOrder R} {partial_order_R : PartialOrder eq R} {total_R : Total R} :
+  ∀ (l_1 l_2 : list A),
+  (∀ x, List.In x l_1 ↔ List.In x l_2) →
+  list_sorted_nodup l_1 →
+  list_sorted_nodup l_2 →
+  l_1 = l_2.
+Proof.
+  intros l_1 l_2 H_in H_l_1 H_l_2. revert l_2 H_in H_l_2; induction l_1 as [| x_1 l_1' IH]; intros l_2 H_in H_l_2.
+  - destruct l_2 as [| x_2 l_2'].
+    + auto.
+    + specialize (H_in x_2). simpl in H_in. ltac1:(intuition auto).
+  - destruct l_2 as [| x_2 l_2'].
+    + specialize (H_in x_1). simpl in H_in. ltac1:(intuition auto).
+    + simpl in H_in, H_l_1, H_l_2. destruct l_1' as [| y_1 l_1''], l_2' as [| y_2 l_2''].
+      * f_equal. specialize (H_in x_2). simpl in H_in. ltac1:(intuition auto).
+      * simpl in H_in. specialize (H_in x_2) as H_1. specialize (H_in y_2) as H_2.
+        assert (H : x_2 = y_2). {
+          clear - H_1 H_2. apply proj2 in H_1. apply proj2 in H_2. ltac1:(intuition congruence).
+        }
+        subst y_2. assert (H : (x_2 ≤ x_2)%le) by reflexivity. clear - H_l_2 H; ltac1:(intuition auto).
+      * simpl in H_in. specialize (H_in x_1) as H_1. specialize (H_in y_1) as H_2.
+        assert (H : x_1 = y_1). {
+          clear - H_1 H_2. apply proj1 in H_1. apply proj1 in H_2. ltac1:(intuition congruence).
+        }
+        subst y_1. assert (H : (x_1 ≤ x_1)%le) by reflexivity. clear - H_l_1 H; ltac1:(intuition auto).
+      * destruct H_l_1 as (H_x_1_y_1 & H_y_1_x_1 & H_l_1'), H_l_2 as (H_x_2_y_2 & H_y_2_x_2 & H_l_2').
+        assert (H_x_1_x_2 : x_1 = x_2). {
+          destruct (classic (x_1 ≤ x_2)%le) as [H_x_1_x_2 | H_x_1_x_2], (classic (x_2 ≤ x_1)%le) as [H_x_2_x_1 | H_x_2_x_1].
+          - apply partial_order_equivalence. split; auto.
+          - assert (H : ¬ List.In x_1 (y_2 :: l_2'')). {
+            apply list_sorted_nodup_impl_not_list_in.
+            - auto.
+            - apply transitivity with x_2; auto.
+            - intros H_1. apply H_y_2_x_2. apply transitivity with x_1; auto.
+          }
+          specialize (H_in x_1). ltac1:(intuition auto).
+          - assert (H : ¬ List.In x_2 (y_1 :: l_1'')). {
+              apply list_sorted_nodup_impl_not_list_in.
+              - auto.
+              - apply transitivity with x_1; auto.
+              - intros H_1. apply H_y_1_x_1. apply transitivity with x_2; auto.
+            }
+            specialize (H_in x_2). ltac1:(intuition auto).
+          - exfalso. destruct (totality x_1 x_2); auto.
+        }
+        subst x_2.
+        assert (H_1 : ¬ List.In x_1 (y_1 :: l_1'')). {
+          apply list_sorted_nodup_impl_not_list_in; auto.
+        }
+        assert (H_2 : ¬ List.In x_1 (y_2 :: l_2'')). {
+          apply list_sorted_nodup_impl_not_list_in; auto.
+        }
+        assert (H_in' : ∀ x, List.In x (y_1 :: l_1'') ↔ List.In x (y_2 :: l_2'')). {
+          intros x. specialize (H_in x). destruct (classic (x_1 = x)) as [<- | H_x_1_x]; ltac1:(intuition auto).
+        }
+        specialize (IH H_l_1' _ H_in' H_l_2'). injection IH as <- IH. f_equal; f_equal; auto.
+Qed.
+
+Lemma list_sorted_nodup_list_filter {A} {R : A → A → Prop} {pre_order_R : PreOrder R} {partial_order_R : PartialOrder eq R} {total_R : Total R} :
+  ∀ f (l : list A),
+  list_sorted_nodup l →
+  list_sorted_nodup (List.filter f l).
+Proof.
+  intros f l H_l. enough (H : list_sorted_nodup (List.filter f l) ∧ ∀ x l' y l_f', l = x :: l' → List.filter f l = y :: l_f' → (x ≤ y)%le).
+  - ltac1:(intuition auto).
+  - induction l as [| x l' IH].
+    + simpl. ltac1:(intuition congruence).
+    + simpl. destruct (f x); simpl in H_l |- *; destruct l' as [| y l''].
+      * simpl. split.
+        -- auto.
+        -- intros ? ? ? ? H_1 H_2; injection H_1 as <- <-; injection H_2 as <- <-. reflexivity.
+      * destruct H_l as (H_x_y & H_y_x & H_l'). specialize (IH H_l') as (IH_1 & IH_2). remember (List.filter f (y :: l'')) as l_f' eqn:H_l_f'. destruct l_f' as [| z l_f''].
+        -- split.
+           ++ auto.
+           ++ intros ? ? ? ? H_1 H_2; injection H_1 as <- <-; injection H_2 as <- <-. reflexivity.
+        -- specialize (IH_2 y l'' z l_f'' eq_refl eq_refl). split > [repeat split |].
+           ++ apply transitivity with y; auto.
+           ++ intros H_z_y. apply H_y_x. apply transitivity with z; auto.
+           ++ auto.
+           ++ intros ? ? ? ? H_1 H_2; injection H_1 as <- <-; injection H_2 as <- <-. reflexivity.
+      * simpl. split.
+        -- auto.
+        -- congruence.
+      * destruct H_l as (H_x_y & H_y_x & H_l'). specialize (IH H_l') as (IH_1 & IH_2). split.
+        -- auto.
+        -- intros ? ? z l_f'' H_1 H_2; injection H_1 as <- <-. specialize (IH_2 y l'' z l_f'' eq_refl H_2).
+           apply transitivity with y; auto.
+Qed.
+
+Definition list_remove {A} {dec_eq_A : EqDec A eq} (x : A) l :=
+  List.filter (λ y, negb (` (bool_of_sumbool (y == x)))) l.
+
+Lemma list_In_list_remove {A} {dec_eq_A : EqDec A eq} :
+  ∀ (x : A) l y,
+  List.In y (list_remove x l) ↔ List.In y l ∧ y ≠ x.
+Proof.
+  intros x l y. unfold list_remove. rewrite List.filter_In. destruct (y == x) as [<- | H_y_x]; simpl.
+  - ltac1:(intuition congruence).
+  - ltac1:(intuition auto).
+Qed.
+
+Lemma list_sorted_nodup_list_remove {A} {dec_eq_A : EqDec A eq} {R : A → A → Prop} {pre_order_R : PreOrder R} {partial_order_R : PartialOrder eq R} {total_R : Total R} {dec_le_R : DecLe R} :
+  ∀ (x : A) l,
+  list_sorted_nodup l →
+  list_sorted_nodup (list_remove x l).
+Proof.
+  intros x l H_l. apply list_sorted_nodup_list_filter. auto.
+Qed.
 
 Inductive mem_index {A} (a : A) : list A → Type :=
   | MIO : ∀ l', mem_index a (a :: l')
@@ -43,41 +465,186 @@ Arguments MIS {A a b l'}.
 
 Check MIS (MIS (MIS MIO)).
 
-Definition stabilizing {A B} (f : A → B) :=
-  ∃ l b, ∀ a, List.In a l ∨ f a = b.
+Definition stabilizing {A B} (f : A → B) keys :=
+  ¬ inhabited A ∨ ∃ b, ∀ a, List.In a keys ∨ f a = b.
 
 Record stabilizing_fun A B := {
   stabilizing_fun_f :> A → B;
-  stabilizing_fun_stabilizing_f : stabilizing stabilizing_fun_f;
+  stabilizing_fun_keys : list A;
+  stabilizing_fun_default : option B;
+  stabilizing_fun_stabilizing_f : stabilizing stabilizing_fun_f stabilizing_fun_keys;
 }.
 Arguments stabilizing_fun_f {A B}.
+Arguments stabilizing_fun_keys {A B}.
+Arguments stabilizing_fun_default {A B}.
 Arguments stabilizing_fun_stabilizing_f {A B}.
 
 Notation "A  '→₀'  B" := (stabilizing_fun A B) (at level 99, right associativity) : type_scope.
 
-Lemma injective_stabilizing_fun_f {A B} :
-  ∀ f g : A →₀ B, stabilizing_fun_f f = stabilizing_fun_f g → f = g.
+Lemma irrelevant_stabilizing_fun {A B} :
+  ∀ f g : A →₀ B,
+  stabilizing_fun_f f = stabilizing_fun_f g →
+  stabilizing_fun_keys f = stabilizing_fun_keys g →
+  stabilizing_fun_default f = stabilizing_fun_default g →
+  f = g.
 Proof.
-  intros f g H. destruct f as [f stabilizing_f], g as [g stabilizing_g].
-  simpl in H. destruct H. f_equal. apply proof_irrelevance.
+  intros f g H_f H_keys H_default. destruct f as [f f_keys f_default stabilizing_f], g as [g g_keys g_default stabilizing_g].
+  simpl in H_f, H_keys, H_default. destruct H_f, H_keys, H_default. f_equal. apply proof_irrelevance.
+Qed.
+
+Definition stabilizing_fun_canonical {A B} {R : A → A → Prop} {pre_order_R : PreOrder R} (f : A →₀ B) :=
+  list_sorted_nodup (stabilizing_fun_keys f) ∧
+  match stabilizing_fun_default f with
+  | None => inhabited (finite A) ∧ ∀ a, List.In a (stabilizing_fun_keys f)
+  | Some b => ¬ inhabited (finite A) ∧ ∀ a, f a ≠ b ↔ List.In a (stabilizing_fun_keys f)
+  end.
+
+#[program]
+Definition stabilizing_fun_canonize {A B} {dec_finite_A : DecFinite A} {R : A → A → Prop} {pre_order_R : PreOrder R} {partial_order_R : PartialOrder eq R} {total_R : Total R} {dec_le_R : DecLe R} {dec_eq_B : EqDec B eq} (f : A →₀ B) := {|
+  stabilizing_fun_f := stabilizing_fun_f f;
+  stabilizing_fun_keys :=
+    match @dec_finite A _ with
+    | inl finite_A => list_sort_nodup (` finite_A)
+    | inr infinite_A =>
+      list_sort_nodup (
+        List.filter
+          (λ a, negb (` (bool_of_sumbool (f a == f (` (infinite_A (stabilizing_fun_keys f)))))))
+          (stabilizing_fun_keys f)
+      )
+    end;
+  stabilizing_fun_default :=
+    match @dec_finite A _ with
+    | inl _ => None
+    | inr infinite_A => Some (f (` (infinite_A (stabilizing_fun_keys f))))
+    end;
+|}.
+Next Obligation.
+  intros A B dec_finite_A R pre_order_R partial_order_R total_R dec_le_R dec_eq_B f. destruct f as [f f_keys f_default stabilizing_f].
+  unfold stabilizing in stabilizing_f |- *. simpl. destruct (@dec_finite A _) as [(list_A & H_list_A) | infinite_A].
+  - simpl. destruct (classic (inhabited A)) as [[a_any] | H_A].
+    + right. exists (f a_any). intros a. left. rewrite list_In_list_sort_nodup. auto.
+    + left. auto.
+  - destruct stabilizing_f as [H_A | (b & H_b)].
+    + left. auto.
+    + ltac1:(replace (f (` (infinite_A f_keys))) with b; revgoals). {
+        destruct (infinite_A f_keys) as (a' & H_a'). simpl. specialize (H_b a'). ltac1:(intuition congruence).
+      }
+      right. exists b. intros a. rewrite list_In_list_sort_nodup, List.filter_In. destruct (H_b a) as [H_a | <-].
+      * destruct (f a == b) as [<- | H_f_a].
+        -- right. auto.
+        -- left. simpl. repeat split. auto.
+      * right. auto.
+Qed.
+
+Lemma stabilizing_fun_canonical_stabilizing_fun_canonize {A B} {dec_finite_A : DecFinite A} {R : A → A → Prop} {pre_order_R : PreOrder R} {partial_order_R : PartialOrder eq R} {total_R : Total R} {dec_le_R : DecLe R} {dec_eq_B : EqDec B eq} :
+  ∀ f : A →₀ B,
+  stabilizing_fun_canonical (stabilizing_fun_canonize f).
+Proof.
+  intros f. unfold stabilizing_fun_canonize, stabilizing_fun_canonical. destruct f as [f f_keys f_default stabilizing_f]. simpl. destruct (@dec_finite A _) as [(list_A & H_list_A) | infinite_A].
+  - simpl. split > [| split].
+    + apply list_sorted_nodup_list_sort_nodup.
+    + exists. exists list_A. auto.
+    + intros a. rewrite list_In_list_sort_nodup. auto.
+  - simpl. split > [| split].
+    + apply list_sorted_nodup_list_sort_nodup.
+    + rewrite not_inhabited_finite_equiv_not_inhabited_infinite. exists. auto.
+    + intros a. rewrite list_In_list_sort_nodup, List.filter_In. destruct stabilizing_f as [H_A | (b & H_b)].
+      * exfalso. apply H_A. exists. auto.
+      * ltac1:(replace (f (` (infinite_A f_keys))) with b; revgoals). {
+          destruct (infinite_A f_keys) as (a' & H_a'). simpl. specialize (H_b a'). ltac1:(intuition congruence).
+        }
+        specialize (H_b a). destruct (f a == b) as [<- | H_f_a]; simpl; ltac1:(intuition (auto; congruence)).
+Qed.
+
+Lemma stabilizing_fun_canonical_impl_canonical {A B} {R : A → A → Prop} {pre_order_R : PreOrder R} {partial_order_R : PartialOrder eq R} {total_R : Total R} :
+  ∀ f g : A →₀ B,
+  stabilizing_fun_f f = stabilizing_fun_f g →
+  stabilizing_fun_canonical f →
+  stabilizing_fun_canonical g →
+  f = g.
+Proof.
+  intros f g H_f canonical_f canonical_g. unfold stabilizing_fun_canonical in canonical_f, canonical_g.
+  destruct f as [f f_keys f_default stabilizing_f], g as [g g_keys g_default stabilizing_g]. simpl in H_f, canonical_f, canonical_g.
+  assert (H_keys_default : f_keys = g_keys ∧ f_default = g_default). {
+    destruct f_default as [f_b |], g_default as [g_b |].
+    + destruct canonical_f as (H_f_keys & H_f_A & H_f_a), canonical_g as (H_g_keys & H_g_A & H_g_a).
+      assert (H_b : f_b = g_b). {
+        apply NNPP. intros H_f_b_g_b. apply H_f_A. exists. exists (f_keys ++ g_keys). intros a.
+        specialize (H_f_a a). specialize (H_g_a a). specialize (@equal_f _ _ _ _ H_f a) as H_f'.
+        rewrite List.in_app_iff. destruct (classic (f a = f_b)) as [<- | H_f_b], (classic (g a = g_b)) as [<- | H_g_b].
+        - exfalso. auto.
+        - right. rewrite <- H_g_a. auto.
+        - left. rewrite <- H_f_a. auto.
+        - left. rewrite <- H_f_a. auto.
+      }
+      assert (H_keys : ∀ a, List.In a f_keys ↔ List.In a g_keys). {
+        intros a. specialize (H_f_a a). specialize (H_g_a a). specialize (@equal_f _ _ _ _ H_f a) as H_f'. rewrite <- H_f_a, <- H_g_a. ltac1:(intuition congruence).
+      }
+      split.
+      * apply list_sorted_nodup_impl_canonical; auto.
+      * f_equal. auto.
+    + destruct canonical_f as (H_f_keys & H_f_A & H_f_a). exfalso. ltac1:(intuition auto).
+    + destruct canonical_g as (H_g_keys & H_g_A & H_g_a). exfalso. ltac1:(intuition auto).
+    + split.
+      * destruct canonical_f as (H_f_keys & H_f_A & H_f_a), canonical_g as (H_g_keys & H_g_A & H_g_a).
+        apply list_sorted_nodup_impl_canonical; ltac1:(intuition auto).
+      * auto.
+  }
+  apply irrelevant_stabilizing_fun; simpl.
+  - auto.
+  - ltac1:(intuition auto).
+  - ltac1:(intuition auto).
 Qed.
 
 #[program]
-Definition stabilizing_fun_const {A B} b : A →₀ B := {|
+Definition stabilizing_fun_const {A B} {dec_finite_A : DecFinite A} {R : A → A → Prop} {pre_order_R : PreOrder R} {partial_order_R : PartialOrder eq R} {total_R : Total R} {dec_le_R : DecLe R} b : A →₀ B := {|
   stabilizing_fun_f := λ _, b;
+  stabilizing_fun_keys :=
+    match @dec_finite A _ with
+    | inl finite_A => list_sort_nodup (` finite_A)
+    | inr _ => []
+    end;
+  stabilizing_fun_default :=
+    if @dec_finite A _ then
+      None
+    else
+      Some b;
 |}.
 Next Obligation.
-  intros A B b. exists [], b. intros a. auto.
+  intros A B dec_finite_A R pre_order_R partial_order_R total_R dec_le_R b. unfold stabilizing.
+  destruct (@dec_finite A _) as [(list_A & H_list_A) | _].
+  - simpl. right. exists b. intros a. rewrite list_In_list_sort_nodup. ltac1:(intuition auto).
+  - simpl. right. exists b. right. auto.
 Qed.
 
 #[program]
-Definition stabilizing_fun_update {A B} `{equiv : Equivalence A eq} `{dec_equiv : @EqDec A eq equiv} (f : A →₀ B) a b := {|
+Definition stabilizing_fun_update {A B} {dec_finite_A : DecFinite A} {dec_eq_A : EqDec A eq} {R : A → A → Prop} {pre_order_R : PreOrder R} {partial_order_R : PartialOrder eq R} {total_R : Total R} {dec_le_R : DecLe R} {dec_eq_B : EqDec B eq} (f : A →₀ B) a b := {|
   stabilizing_fun_f := λ a', if a' == a then b else f a';
+  stabilizing_fun_keys :=
+    match @dec_finite A _ with
+    | inl _ => list_insert_nodup a (stabilizing_fun_keys f)
+    | inr infinite_A =>
+      if b == f (` (infinite_A (stabilizing_fun_keys f))) then
+        list_remove a (stabilizing_fun_keys f)
+      else
+        list_insert_nodup a (stabilizing_fun_keys f)
+    end;
+  stabilizing_fun_default := stabilizing_fun_default f;
 |}.
 Next Obligation.
-  intros A B equiv dec_equiv f a b. destruct f as [f (l & b' & H_f)]. exists (a :: l), b'. intros a'. simpl. destruct (a' == a) as [H_a' | H_a'].
-  - left. left. auto.
-  - specialize (H_f a'). destruct H_f; auto.
+  intros A B dec_finite_A dec_eq_A R pre_order_R partial_order_R total_R dec_le_R dec_eq_B f a b. destruct f as [f f_keys f_default stabilizing_f].
+  simpl. unfold stabilizing in stabilizing_f |- *. destruct stabilizing_f as [H | (b_stabilizing & H_b_stabilizing)].
+  - left. auto.
+  - right. exists b_stabilizing. intros a'. destruct (@dec_finite A _) as [(list_A & H_list_A) | infinite_A].
+    + rewrite list_In_list_insert_nodup. destruct (a' == a) as [-> | _].
+      * left. right. auto.
+      * specialize (H_b_stabilizing a'). ltac1:(intuition auto).
+    + ltac1:(replace (f (` (infinite_A f_keys))) with b_stabilizing; revgoals). {
+        destruct (infinite_A f_keys) as (a'' & H_a''). simpl. specialize (H_b_stabilizing a''). ltac1:(intuition congruence).
+      }
+      destruct (b == b_stabilizing) as [-> | H_b].
+      * rewrite list_In_list_remove. specialize (H_b_stabilizing a'). destruct (a' == a) as [-> | H_a']; ltac1:(intuition auto).
+      * rewrite list_In_list_insert_nodup. specialize (H_b_stabilizing a'). destruct (a' == a) as [-> | H_a']; ltac1:(intuition auto).
 Qed.
 
 Declare Scope stabilizing_fun_scope.
@@ -85,5 +652,51 @@ Delimit Scope stabilizing_fun_scope with stabilizing_fun.
 Bind Scope stabilizing_fun_scope with stabilizing_fun.
 Open Scope stabilizing_fun_scope.
 
-Notation "'_'  '↦₀'  b" := (stabilizing_fun_const b) (at level 70) : stabilizing_fun_scope.
-Notation "a  '↦₀'  b ','  f" := (stabilizing_fun_update f a b) (at level 70, f at level 200) : stabilizing_fun_scope.
+Notation "'_' '↦₀' b" := (stabilizing_fun_const b) (at level 10, b at level 69, format "'[' '_'  '↦₀'  b ']'") : stabilizing_fun_scope.
+Notation "( '_' : A ) '↦₀' b" := (@stabilizing_fun_const A _ _ _ _ _ _ _ b) (at level 0, b at level 69, format "'[' '(' '_'  ':'  A ')'  '↦₀'  b ']'") : stabilizing_fun_scope.
+Notation "a '↦₀' b ',' f" := (stabilizing_fun_update f a b) (at level 70, b at level 69, f at level 200, format "'[' a  '↦₀'  b ',' '/' f ']'") : stabilizing_fun_scope.
+
+Lemma stabilizing_fun_canonical_stabilizing_fun_const {A B} {dec_finite_A : DecFinite A} {R : A → A → Prop} {pre_order_R : PreOrder R} {partial_order_R : PartialOrder eq R} {total_R : Total R} {dec_le_R : DecLe R} :
+  ∀ b : B,
+  stabilizing_fun_canonical ((_ : A) ↦₀ b).
+Proof.
+  intros b. unfold stabilizing_fun_canonical. simpl. destruct (@dec_finite A _) as [(list_A & H_list_A) | infinite_A].
+  - simpl. split > [| split].
+    + apply list_sorted_nodup_list_sort_nodup.
+    + exists. exists list_A. auto.
+    + intros a. rewrite list_In_list_sort_nodup. auto.
+  - simpl. split > [| split].
+    + auto.
+    + rewrite not_inhabited_finite_equiv_not_inhabited_infinite. exists. auto.
+    + ltac1: (intuition congruence).
+Qed.
+
+Lemma stabilizing_fun_canonical_stabilizing_fun_update {A B} {dec_finite_A : DecFinite A} {dec_eq_A : EqDec A eq} {R : A → A → Prop} {pre_order_R : PreOrder R} {partial_order_R : PartialOrder eq R} {total_R : Total R} {dec_le_R : DecLe R} {dec_eq_B : EqDec B eq} :
+  ∀ (f : A →₀ B) a b,
+  stabilizing_fun_canonical f →
+  stabilizing_fun_canonical (a ↦₀ b, f).
+Proof.
+  intros f a b canonical_f. unfold stabilizing_fun_canonical in canonical_f |- *. destruct f as [f f_keys f_default stabilizing_f]. simpl in canonical_f |- *. destruct (@dec_finite A _) as [(list_A & H_list_A) | infinite_A], f_default as [b_default |], canonical_f as (H_f_keys & H_f_A & H_f_a).
+  - exfalso. apply H_f_A. exists. exists list_A. auto.
+  - split > [| split].
+    + apply list_sorted_nodup_list_insert_nodup. auto.
+    + exists. exists list_A. auto.
+    + intros a'. rewrite list_In_list_insert_nodup. left. auto.
+  - ltac1:(replace (f (` (infinite_A f_keys))) with b_default; revgoals). {
+      destruct (infinite_A f_keys) as (a'' & H_a''). simpl. specialize (H_f_a a''). apply NNPP. ltac1:(intuition auto).
+    }
+    destruct (b == b_default) as [-> | H_b].
+    + split > [| split].
+      * apply list_sorted_nodup_list_remove. auto.
+      * rewrite not_inhabited_finite_equiv_not_inhabited_infinite. exists. auto.
+      * intros a'. rewrite list_In_list_remove. destruct (a' == a) as [H_a' | H_a'].
+        -- ltac1:(intuition auto).
+        -- specialize (H_f_a a'). ltac1:(intuition auto).
+    + split > [| split].
+      * apply list_sorted_nodup_list_insert_nodup. auto.
+      * rewrite not_inhabited_finite_equiv_not_inhabited_infinite. exists. auto.
+      * intros a'. rewrite list_In_list_insert_nodup. destruct (a' == a) as [H_a' | H_a'].
+        -- ltac1:(intuition auto).
+        -- specialize (H_f_a a'). ltac1:(intuition congruence).
+  - exfalso. destruct H_f_A as [H_f_A]. apply (not_finite_and_infinite A); auto.
+Qed.
