theories/PCFm.v
@@ -4,16 +4,16 @@ From PCF Require Import Types.
 
 Inductive termₘ μ : list type → type → Type :=
   | Oₘ : ∀ Γ, termₘ μ Γ ι
-  | predₘ : ∀ Γ, termₘ μ Γ (ι ⇒ ι)
-  | succₘ : ∀ Γ, termₘ μ Γ (ι ⇒ ι)
+  | Pₘ : ∀ Γ, termₘ μ Γ (ι ⇒ ι)
+  | Sₘ : ∀ Γ, termₘ μ Γ (ι ⇒ ι)
   | switchₘ : ∀ Γ, termₘ μ Γ ι → (Zm μ →₀ termₘ μ Γ ι) → termₘ μ Γ ι
   | fixₘ : ∀ Γ α, termₘ μ Γ ((α ⇒ α) ⇒ α)
   | Varₘ : ∀ Γ α, mem_index α Γ → termₘ μ Γ α
   | Appₘ : ∀ Γ α β, termₘ μ Γ (α ⇒ β) → termₘ μ Γ α → termₘ μ Γ β
   | Absₘ : ∀ Γ α β, termₘ μ (β :: Γ) α → termₘ μ Γ (β ⇒ α).
 Arguments Oₘ {μ Γ}.
-Arguments predₘ {μ Γ}.
-Arguments succₘ {μ Γ}.
+Arguments Pₘ {μ Γ}.
+Arguments Sₘ {μ Γ}.
 Arguments switchₘ {μ Γ}.
 Arguments fixₘ {μ Γ}.
 Arguments Varₘ {μ Γ}.
@@ -23,7 +23,7 @@ Arguments Absₘ {μ Γ α}.
 Notation "s  '$ₘ'  t" := (Appₘ s t) (at level 40, left associativity).
 Notation "'λₘ:'  α ','  s" := (Absₘ α s) (at level 35, s at level 200).
 
-Check (λₘ: ι, λₘ: ι, Varₘ ι (MIS MIO)) $ₘ (succₘ $ₘ Varₘ ι MIO) $ₘ Oₘ.
+Check (λₘ: ι, λₘ: ι, Varₘ ι (MIS MIO)) $ₘ (Sₘ $ₘ Varₘ ι MIO) $ₘ Oₘ.
 (* Check (λₘ: ι, λₘ: ι, Varₘ ι (MIS MIO)) $ₘ (λₘ: ι, Varₘ ι MIO). *)
 
-Check λₘ: ι, switchₘ (Varₘ ι MIO) (Zm_of_Z 0 ↦₀ succₘ $ₘ (succₘ $ₘ Oₘ), Zm_of_Z 1 ↦₀ Oₘ, _ ↦₀ succₘ $ₘ Oₘ).
+(* Check λₘ: ι, switchₘ (Varₘ ι MIO) (Zm_of_Z 0 ↦₀ Sₘ $ₘ (Sₘ $ₘ Oₘ), Zm_of_Z 1 ↦₀ Oₘ, _ ↦₀ Sₘ $ₘ Oₘ). *)
