theories/Zm.v
@@ -4,7 +4,7 @@ Definition Zm_in_bounds (μ : nat) (n : Z) :=
   (0 ≤ n < Z.of_nat μ)%Z.
 
 Definition Zm_canonical (μ : nat) (n : Z) :=
-  ∀ m : Z, Zm_in_bounds μ (n + Z.of_nat μ * m)%Z → m = 0%Z.
+  ∀ m : Z, Zm_in_bounds μ (n + m * Z.of_nat μ)%Z → m = 0%Z.
 
 Record Zm μ := {
   Zm_n : Z;
@@ -19,8 +19,10 @@ Bind Scope Zm_scope with Zm.
 
 Notation "'mod'  n" := {| Zm_n := n |} (at level 35, only printing) : Zm_scope.
 
-Lemma injective_Zm_n {μ} :
-  ∀ n m : Zm μ, Zm_n n = Zm_n m → n = m.
+Lemma irrelevant_Zm {μ} :
+  ∀ n m : Zm μ,
+  Zm_n n = Zm_n m →
+  n = m.
 Proof.
   intros n m H. destruct n as [n canonical_n], m as [m canonical_m].
   simpl in H. destruct H. f_equal. apply proof_irrelevance.
@@ -30,23 +32,38 @@ Lemma Zm_eq_dec {μ} :
   ∀ n m : Zm μ, {n = m} + {n ≠ m}.
 Proof.
   intros n m. destruct (Z.eq_dec (Zm_n n) (Zm_n m)) as [H_n_m | H_n_m].
-  - left. apply injective_Zm_n. auto.
+  - left. apply irrelevant_Zm. auto.
   - right. intros <-. auto.
 Qed.
 
 Instance dec_eq_Zm {μ} : EqDec (Zm μ) eq := Zm_eq_dec.
+
+Lemma Zm_in_bounds_impl_mod :
+  ∀ μ n,
+  Zm_in_bounds μ n →
+  (n mod Z.of_nat μ)%Z = n.
+Proof.
+  intros μ n H. apply Zmod_small. auto.
+Qed.
 
 #[program]
 Definition Zm_of_Z {μ} (n : Z) : Zm μ := {|
   Zm_n := (n mod Z.of_nat μ)%Z;
 |}.
 Next Obligation.
-  intros μ n. Locate "_ mod _". Search Z.modulo.
-Admitted.
+  intros μ n m H_m. remember (n mod Z.of_nat μ + m * Z.of_nat μ)%Z as k eqn:H_k.
+  pose (H'_k := H_k). rewrite <- (Zm_in_bounds_impl_mod μ) in H'_k by (subst k; auto).
+  rewrite Z_mod_plus_full in H'_k. rewrite Zmod_mod in H'_k. rewrite H'_k in H_k; clear H'_k.
+  rewrite Z.add_comm in H_k. apply (Zplus_eq_compat _ _ (- (n mod Z.of_nat μ))%Z (- (n mod Z.of_nat μ))%Z) in H_k.
+  - rewrite <- Z.add_assoc in H_k. rewrite Z.add_opp_diag_r in H_k. rewrite Z.add_0_r in H_k.
+    symmetry in H_k. apply Zmult_integral in H_k. unfold Zm_in_bounds in H_m. destruct H_k as [H_k | H_k]; lia.
+  - reflexivity.
+Qed.
 
 Lemma idempotent_Zm_of_Z {μ} :
   ∀ n, @Zm_of_Z μ (@Zm_n μ (Zm_of_Z n)) = Zm_of_Z n.
 Proof.
-Admitted.
+  intros n. apply irrelevant_Zm. simpl. rewrite Zmod_mod. auto.
+Qed.
 
 Compute Zm_of_Z 7 : Zm 3.
